Slight progress on multi-arg introduction

new-backend/clos_mtiScript.sml
@@ -18,16 +18,16 @@ val cEval_length_imp = Q.prove (
  rfs []);
 
 val collect_args_def = Define `
-(collect_args num_args (Fn loc fvs num_args' e) =
+(collect_args max_app num_args (Fn loc fvs num_args' e) =
   if num_args + num_args' ≤ max_app then
-    collect_args (num_args + num_args') e
+    collect_args max_app (num_args + num_args') e
   else 
     (max_app, Fn loc fvs (num_args + num_args' - max_app) e)) ∧
-(collect_args num_args e = (num_args, e))`;
+(collect_args max_app num_args e = (num_args, e))`;
 
 val collect_args_size = Q.prove (
-`!num_args e num_args' e'.
-  (num_args', e') = collect_args num_args e ⇒ 
+`!max_app num_args e num_args' e'.
+  (num_args', e') = collect_args max_app num_args e ⇒ 
   num_args' + clos_exp_size e' ≤ num_args + clos_exp_size e`,
  ho_match_mp_tac (fetch "-" "collect_args_ind") >>
  rw [collect_args_def, clos_exp_size_def] >>
@@ -55,11 +55,11 @@ val intro_multi_def = tDefine "intro_multi"`
 (intro_multi [App loc e es] =
   [App loc (HD (intro_multi [e])) (intro_multi es)]) ∧
 (intro_multi [Fn loc fvs num_args e] =
-  let (num_args', e') = collect_args num_args e in
+  let (num_args', e') = collect_args max_app num_args e in
     [Fn loc fvs num_args' (HD (intro_multi [e']))]) ∧
 (intro_multi [Letrec loc fvs funs e] =
   [Letrec loc fvs (MAP (\(num_args, e). 
-                         let (num_args', e') = collect_args num_args e in
+                         let (num_args', e') = collect_args max_app num_args e in
                            (num_args', HD (intro_multi [e'])))
                        funs)
       (HD (intro_multi [e]))]) ∧
@@ -91,6 +91,17 @@ val clos_val_size_el = Q.prove (
      fs [] >>
      decide_tac));
 
+val exp_rel_def = Define `
+exp_rel (num_args,e) (num_args',e') ⇔
+  num_args ≤ max_app ∧
+  0 < num_args ∧
+  num_args' ≤ max_app ∧
+  0 < num_args' ∧
+  num_args ≤ num_args' ∧
+  ?e''.
+    (num_args',e'') = collect_args num_args' num_args e ∧
+    e' = HD (intro_multi [e''])`;
+
 val (val_rel_rules, val_rel_ind, val_rel_cases) = Hol_reln `
 (!n. 
   val_rel (Number n) (Number n)) ∧
@@ -100,27 +111,20 @@ val (val_rel_rules, val_rel_ind, val_rel_cases) = Hol_reln `
   val_rel (Block n vs) (Block n vs')) ∧
 (!n.
   val_rel (RefPtr n) (RefPtr n)) ∧
-(!num_args' e' e args' args env env'.
-  num_args ≤ max_app ∧
-  0 < num_args ∧
-  (num_args', e') = collect_args num_args e ∧
+(!num_args' e' e args' args env env' loc num_args.
   LIST_REL val_rel args args' ∧
-  LIST_REL val_rel env env'
+  LIST_REL val_rel env env' ∧
+  exp_rel (num_args,e) (num_args',e')
   ⇒
   val_rel (Closure loc args env num_args e) 
-          (Closure loc args' env' num_args' (HD (intro_multi [e'])))) ∧
-(!args args' env env' funs i.
-  EVERY (\(num_args,e). num_args ≤ map_app ∧ 0 < num_args) funs ∧
+          (Closure loc args' env' num_args' e')) ∧
+(!args args' env env' funs funs' i.
   LIST_REL val_rel args args' ∧
-  LIST_REL val_rel env env'
+  LIST_REL val_rel env env' ∧
+  LIST_REL exp_rel funs funs'
   ⇒
   val_rel (Recclosure loc args env funs i)
-          (Recclosure loc args' env'
-             (MAP (\(num_args, e). 
-                         let (num_args', e') = collect_args num_args e in
-                           (num_args', HD (intro_multi [e'])))
-                  funs)
-             i))`;
+          (Recclosure loc args' env' funs' i))`;
 
 val (res_rel_rules, res_rel_ind, res_rel_cases) = Hol_reln `
 (!vs.
@@ -139,23 +143,32 @@ val (ref_v_rel_rules, ref_v_rel_ind, ref_v_rel_cases) = Hol_reln `
   ⇒
   ref_v_rel (ValueArray vs) (ValueArray vs'))`;
 
-val state_comp_def = Define `
-state_comp (s:clos_state) s' ⇔
+val state_rel_def = Define `
+state_rel (s:clos_state) s' ⇔
   LIST_REL (OPTION_REL val_rel) s.globals s'.globals ∧
   fmap_rel ref_v_rel s.refs s'.refs ∧
-  s'.code = (\(n,e). (n, HD (intro_multi [e]))) o_f s.code`;
+  s.clock = s'.clock ∧
+  fmap_rel exp_rel s.code s'.code ∧
+  s.output = s'.output ∧
+  s.restrict_envs = s'.restrict_envs`;
 
-val lookup_vars_map = Q.prove (
-`!vs env f. lookup_vars vs (MAP f env) = OPTION_MAP (MAP f) (lookup_vars vs env)`,
+val lookup_vars_list_rel = Q.prove (
+`!vs env env' f. 
+  LIST_REL f env env'
+  ⇒
+  OPTION_REL (LIST_REL f) (lookup_vars vs env) (lookup_vars vs env')`,
  Induct_on `vs` >>
  rw [lookup_vars_def] >>
  ect >>
- fs [EL_MAP]);
+ fs [OPTREL_def] >>
+ res_tac >>
+ fs [LIST_REL_EL_EQN] >>
+ metis_tac []);
 
 val collect_args_more = Q.prove (
-`!num_args e num_args' e'.
+`!max_app num_args e num_args' e'.
   num_args ≤ max_app ∧
-  (num_args', e') = collect_args num_args e
+  (num_args', e') = collect_args max_app num_args e
   ⇒
   num_args ≤ num_args' ∧ num_args' ≤ max_app`,
  ho_match_mp_tac (fetch "-" "collect_args_ind") >>
@@ -164,7 +177,32 @@ val collect_args_more = Q.prove (
  res_tac >>
  decide_tac);
 
-val intro_multi_length = Q.prove (
+val collect_args_mono = Q.prove (
+`!num_args4 num_args2 exp num_args3 exp' num_args1.
+  num_args2 ≤ num_args3 ∧
+  num_args3 ≤ num_args1 ∧
+  num_args4 = num_args3 ∧
+  collect_args num_args1 num_args2 exp = (num_args3, exp')
+  ⇒
+  collect_args num_args4 num_args2 exp = (num_args3, exp')`,
+ ho_match_mp_tac (fetch "-" "collect_args_ind") >>
+ rw [collect_args_def] >>
+ rw [] >>
+ fs [NOT_LESS_EQUAL] >>
+ ect >>
+ fs [] >>
+ fs [NOT_LESS_EQUAL] >>
+ rw [] >>
+ TRY (first_x_assum match_mp_tac) >>
+ full_simp_tac (srw_ss()++ARITH_ss) []
+ >- metis_tac [] >>
+ pop_assum mp_tac >>
+ pop_assum (mp_tac o GSYM) >>
+ rw [] >>
+ imp_res_tac collect_args_more >>
+ full_simp_tac (srw_ss()++ARITH_ss) []);
+
+val intro_multi_length = Q.prove ( 
 `!es. LENGTH (intro_multi es) = LENGTH es`,
  recInduct (fetch "-" "intro_multi_ind") >>
  rw [intro_multi_def] >>
@@ -174,9 +212,10 @@ val intro_multi_sing = Q.prove (
 `!e. ?e'. intro_multi [e] = [e']`,
  Cases_on `e` >>
  rw [intro_multi_def] >>
- Cases_on `collect_args n c` >>
+ Cases_on `collect_args max_app n c` >>
  fs []);
 
+ (*
 val (dest_cl_res_rel_rules, dest_cl_res_rel_ind, dest_cl_res_rel_cases) = Hol_reln `
 (!v v'.
   val_rel v v'
@@ -188,7 +227,6 @@ val (dest_cl_res_rel_rules, dest_cl_res_rel_ind, dest_cl_res_rel_cases) = Hol_re
   ⇒
   (dest_cl_res_rel (Full_app e env args) (Full_app (HD (intro_multi [e])) env' args')))`;
 
-  (*
 val dest_closure_thm = Q.prove (
 `!loc f args res f' args' res'.
   dest_closure NONE f args = SOME res ∧
@@ -204,16 +242,33 @@ val dest_closure_thm = Q.prove (
  ect >>
  fs [Once val_rel_cases, dest_cl_res_rel_cases] >>
  rw [] >>
- fs [check_loc_def] >>
+ fs [check_loc_def, exp_rel_def] >>
  imp_res_tac EVERY2_LENGTH >>
- imp_res_tac collect_args_more >>
  TRY (`n - LENGTH l ≤ LENGTH args'` by decide_tac) >>
  TRY (`n' - LENGTH l' ≤ LENGTH args` by decide_tac) >>
  rw [DROP_REVERSE, TAKE_REVERSE, LASTN_MAP, ETA_THM, BUTLASTN_MAP] >>
  fs [] >>
- TRY decide_tac >>
  rev_full_simp_tac (srw_ss()++ARITH_ss) [NOT_LESS] >>
+ rw [] >>
+
+ Cases_on `f` >>
+ fs []
+ Cases_on `f'` >>
+ fs [] >>
+ fs [Once val_rel_cases] >>
  rw []
+ Cases_on `¬(LENGTH args + LENGTH l < n)` >>
+ fs []
+
+ metis_tac [EVERY2_APPEND]
+
+ imp_res_tac EVERY2_LENGTH >>
+
+ simp []
+ fs [check_loc_def]
+ `n ≤ n'` by fs [exp_rel_def] >>
+ rw []
+
 
  Cases_on `c'` >>
  fs [intro_multi_def, collect_args_def]
@@ -221,27 +276,39 @@ val dest_closure_thm = Q.prove (
  fs []
 
 val intro_multi_correct = Q.prove (
-`(!tmp es env s1 res s2.
+`(!tmp es env s1 res s2 s1' env'.
    tmp = (es,env,s1) ∧
    cEval tmp = (res, s2) ∧
-   res ≠ Error
+   res ≠ Error ∧
+   LIST_REL val_rel env env' ∧
+   state_rel s1 s1'
    ⇒
-   cEval (intro_multi es, MAP val_comp env, state_comp s1) = (res_comp res, state_comp s2)) ∧
- (!loc_opt func args s1 res s2.
+   ?res' s2'.
+     state_rel s2 s2' ∧
+     res_rel res res' ∧
+     cEval (intro_multi es, env', s1') = (res', s2')) ∧
+ (!loc_opt func args s1 res s2 func' args' s1'.
    cEvalApp loc_opt func args s1 = (res, s2) ∧
-   res ≠ Error
+   res ≠ Error ∧
+   val_rel func func' ∧
+   LIST_REL val_rel args args' ∧
+   state_rel s1 s1'
    ⇒
-   cEvalApp loc_opt (val_comp func) (MAP val_comp args) (state_comp s1) = (res_comp res, state_comp s2))`,
+   ?res' s2'.
+     state_rel s2 s2' ∧
+     res_rel res res' ∧
+     cEvalApp loc_opt func' args' s1' = (res', s2'))`,
 
  ho_match_mp_tac cEval_ind >>
  rpt strip_tac
  >- (fs [cEval_def, intro_multi_def] >>
-     rw [cEval_def, intro_multi_def, res_comp_def])
+     rw [cEval_def, intro_multi_def, res_rel_cases])
  >- cheat
  >- (fs [cEval_def, intro_multi_def] >>
-     rw [cEval_def, intro_multi_def, res_comp_def] >>
-     fs [] >>
-     rw [res_comp_def, EL_MAP])
+     rw [cEval_def, intro_multi_def] >>
+     imp_res_tac EVERY2_LENGTH >>
+     fs [LIST_REL_EL_EQN] >>
+     rw [res_rel_cases])
  >- cheat
  >- cheat
  >- cheat
@@ -253,40 +320,69 @@ val intro_multi_correct = Q.prove (
      fs [] >>
      ect >>
      fs [] >>
-     rw [res_comp_def] >>
-     fs [state_comp_def, clos_env_def] >>
-     ect >>
-     fs [val_comp_def, lookup_vars_map] >>
-     rw [ETA_THM] >>
-     imp_res_tac collect_args_more  >>
-     decide_tac)
+     rw [] >>
+     `s.restrict_envs = s1'.restrict_envs` by fs [state_rel_def] >>
+     fs [res_rel_cases, clos_env_def]
+     >- (ect >>
+         fs [] >>
+         imp_res_tac lookup_vars_list_rel >>
+         pop_assum (qspec_then `vs` mp_tac) >>
+         rw [OPTREL_def]) >>
+     `LIST_REL val_rel x' x`
+           by (ect >>
+               fs [] >>
+               imp_res_tac lookup_vars_list_rel >>
+               pop_assum (qspec_then `vs` mp_tac) >>
+               rw [OPTREL_def]) >>
+     `?num_args' e'. collect_args max_app num_args exp = (num_args', e')` by metis_tac [pair_CASES] >>
+     simp [] >>
+     `num_args' ≤ max_app ∧ num_args ≤ num_args'` by metis_tac [collect_args_more] >>
+     simp [] >>
+     rw [Once val_rel_cases] >>
+     simp [exp_rel_def] >>
+     qexists_tac `e'` >>
+     rw [] >>
+     metis_tac [collect_args_mono])
  >- cheat
  >- (fs [cEval_def, intro_multi_def] >>
-     rw [cEval_def, intro_multi_def, res_comp_def] >>
+     rw [cEval_def, intro_multi_def] >>
      fs [intro_multi_length] >>
-     ect >>
+     `?res1 s1. cEval (args, env, s) = (res1,s1)` by metis_tac [pair_CASES] >>
      fs [] >>
-     rw [] >>
-     rfs [res_comp_def] >>
-     rw [] >>
+     reverse (Cases_on `res1`) >>
      fs [] >>
-     rfs [] >>
+     rw []
+     >- (res_tac >>
+         rw [] >>
+         fs [res_rel_cases] >>
+         rw [])
+     >- (res_tac >>
+         rw [] >>
+         fs [res_rel_cases] >>
+         rw []) >>
+     `?res2 s2. cEval ([x1], env, s1) = (res2,s2)` by metis_tac [pair_CASES] >>
      `?x1'. intro_multi [x1] = [x1']` by metis_tac [intro_multi_sing] >>
      fs [] >>
-     rfs [] >>
+     reverse (Cases_on `res2`) >>
+     fs [] >>
+     rw [] >>
+     res_tac >>
+     rw [] >>
+     fs [res_rel_cases] >>
+     rw [] >>
+     first_x_assum match_mp_tac >>
+     rw [] >>
+     Cases_on `a'` >>
+     Cases_on `vs'''` >>
+     fs [] >>
      imp_res_tac cEval_length_imp >>
-     fs [] >>
-     Cases_on `a''` >>
-     fs [] >>
-     Cases_on `a` >>
-     fs [] >>
-     metis_tac [])
+     fs [])
  >- cheat
  >- cheat
  >- (fs [cEval_def] >>
      Cases_on `res` >>
-     fs [res_comp_def] >>
-     metis_tac [MAP])
+     fs [res_rel_cases] >>
+     metis_tac [])
 
  >- (fs [cEval_def] >>
      ect >>
